theories/Dot/lr/lr_lemmas.v
@@ -119,6 +119,7 @@ Hint Resolve ctx_id_syn ctx_trans_sub_syn unTLater_ctx_sub_syn
 (** * When is a context weaker than another? While we don't give complete
 rules, we develop some infrastructure to allow "stripping" laters from the
 context. *)
+(* This is specialized to [vnil] because contexts only contain proper types anyway. *)
 Definition ty_sub `{HdlangG: dlangG Σ} T1 T2 := ∀ ρ v, p⟦ T1 ⟧ vnil ρ v -∗ p⟦ T2 ⟧ vnil ρ v.
 Notation "⊨T T1 <: T2" := (ty_sub T1 T2) (at level 74, T1, T2 at next level).
 Typeclasses Opaque ty_sub.
